## Truth Table to Boolean Expression
With a given truth table, we can write out its boolean expression, following these steps
$$f:(x,y,z)\to\{0,1\}$$
**Disjunctive normal form** (DNF) formula:
1. Find all rows of $f = 1$
2. For each row, write down an expression as a clause that only evaluates to the result this row:
   $$A_i \wedge B_i\wedge C_i$$
	- If $x = 0, A_i = \neg x$
	- If $x = 1, A_i = x$
	- Same for all other boolean variables
3. Combine all clauses with OR
4. Change the format

> [!example]
>
> |  x  |  y  |  z  |  f  |  Expression  |
> | :-: | :--: | :-: | :--: | :--: |
> |  0  |  0  |  0  |  1  | $\neg x \wedge \neg y \wedge \neg z$  |
> |  0  |  0  |  1  |  0  |    |
> |  0  |  1  |  0  |  1  |  $\neg x \wedge y \wedge \neg z$ |
> |  0  |  1  |  1  |  0 |    |
> |  1  |  0  |  0  |  1  |  $x \wedge \neg y \wedge \neg z$  |
> |  1  |  0  |  1  |  0  |    |
> |  1  |  1  |  0  |  0  |    |
> |  1  |  1  |  1  |  0  |    |
> Outcome:
> $$\begin{align}f(x,y,z) &= (\neg x \wedge \neg y \wedge \neg z)\vee(\neg x \wedge y \wedge \neg z)\vee (x \wedge \neg y \wedge \neg z)\\&= (x\wedge y)\vee (\neg x\wedge z)\end{align}$$



## Theorem
Any Boolean function can be represented using an expression containing AND, OR and NOT operations.

Any Boolean function can be represented using an expression containing AND and NOT operations.

- Proof: De Morgan's Formula
  $$x\lor y = \neg(\neg x\land \neg y)$$

Any Boolean function can be represented using an expression containing only NAND operation.

## NAND operation
$$x \barwedge y = \neg(A\land B)$$

| x   | y   | NAND |
| --- | --- | ---- |
| 0   | 0   | 1    |
| 0   | 1   | 1    |
| 1   | 0   | 1    |
| 1   | 1   | 0    |

**NOT** through NAND
$$\neg x = x \barwedge x$$
**AND** throught NAND
$$x\land y = \neg(x\barwedge y) = (x\barwedge y)\barwedge (x\barwedge y)$$
